src/ExecutionPlan.v
@@ -8,12 +8,13 @@ From hahn Require Import HahnBase.
 From Coq Require Import Classes.EquivDec.
 From Coq Require Import Classes.RelationClasses.
 
-Require Import Cypher.
-Require Import Semantics.
-Require Import BindingTable.
-Require Import PropertyGraph.
 Require Import Maps.
 Require Import Utils.
+Require Import PropertyGraph.
+Require Import Cypher.
+Require Import BindingTable.
+Require Import Semantics.
+Require Import PatternE.
 Import PartialMap.Notations.
 Import PropertyGraph.
 
@@ -77,6 +78,9 @@ Module ExecutionPlan.
     (* return_all : step1 *)
     Parameter return_all : step1.
 
+    (* traverse (slice : PatternSlice.t) (n_from : Name.t) : step1 *)
+    Parameter traverse : PatternSlice.t -> Name.t -> step1.
+
     Section axioms.
       Variable graph : PropertyGraph.t.
       Variable table : BindingTable.t.
@@ -112,6 +116,11 @@ Module ExecutionPlan.
       Axiom return_all_wf :
         exists table', return_all graph table = Some table'.
 
+      Axiom traverse_wf : forall slice n_from,
+        PropertyGraph.wf graph -> BindingTable.of_type table ty ->
+          PatternSlice.wf ty slice -> ty n_from = Some Value.GVertexT ->
+            exists table', traverse slice n_from graph table = Some table'.
+
       (** If the operation returned some table then the type of the table is correct *)
 
       Axiom scan_vertices_type : forall n,
@@ -133,6 +142,11 @@ Module ExecutionPlan.
         return_all graph table = Some table' ->
           BindingTable.of_type table ty ->
             BindingTable.of_type table' (Rcd.explicit_projT ty).
+
+      Axiom traverse_type : forall slice n_from,
+        traverse slice n_from graph table = Some table' ->
+          BindingTable.of_type table ty ->
+            BindingTable.of_type table' (PatternSlice.type_of ty slice).
 
       (** scan_vertices specification *)
 
@@ -188,6 +202,18 @@ Module ExecutionPlan.
       Axiom return_all_spec' : forall r',
         return_all graph table = Some table' ->
           In r' table' -> exists r, In r table /\ r' = Rcd.explicit_proj r.
+
+      (** traverse specification *)
+
+      Axiom traverse_spec : forall path r r' slice n_from,
+        traverse slice n_from graph table = Some table' ->
+          PathSlice.matches graph r n_from r' path slice ->
+            In r table -> In r' table'.
+
+      Axiom traverse_spec' : forall r' slice n_from,
+        traverse slice n_from graph table = Some table' ->
+          In r' table' -> exists r path, In r table /\
+            PathSlice.matches graph r n_from r' path slice.
     End axioms.
   End Spec.
 
@@ -196,6 +222,7 @@ Module ExecutionPlan.
   | FilterByLabel (mode : FilterMode.t) (n : Name.t) (l : label) (plan : t) 
   | Expand (mode : ExpandMode.t) (n_from n_edge n_to : Name.t) (d : Pattern.direction) (plan : t)
   | ReturnAll (plan : t)
+  | Traverse (slice : PatternSlice.t) (n_from : Name.t) (plan : t)
   .
 
   Fixpoint type_of (plan : t) : BindingTable.T :=
@@ -204,6 +231,7 @@ Module ExecutionPlan.
     | FilterByLabel mode n l plan => type_of plan
     | Expand mode n_from n_edge n_to d plan => n_to |-> Value.GVertexT; n_edge |-> Value.GEdgeT; type_of plan
     | ReturnAll plan => Rcd.explicit_projT (type_of plan)
+    | Traverse slice n_from plan => PatternSlice.type_of (type_of plan) slice
     end.
 
   Lemma type_of_types plan k :
@@ -215,7 +243,7 @@ Module ExecutionPlan.
     all: unfold Rcd.explicit_projT.
     all: autounfold with unfold_pat.
     all: desf.
-    all: auto.
+    all: auto using PatternSlice.type_of__types.
   Qed.
 
   Fixpoint wf (plan : t) :=
@@ -243,6 +271,10 @@ Module ExecutionPlan.
       << Hwf : wf plan >>
     | ReturnAll plan =>
       << Hwf : wf plan >>
+    | Traverse slice n_from plan =>
+      << Htype : type_of plan n_from = Some Value.GVertexT >> /\
+      << Hwf_slice : PatternSlice.wf (type_of plan) slice >> /\
+      << Hwf : wf plan >>
     end.
 
   Module EvalPlan (S : Spec).
@@ -250,11 +282,11 @@ Module ExecutionPlan.
 
     #[local]
     Hint Resolve scan_vertices_type filter_by_label_type
-                expand_type return_all_type : type_axioms.
+                expand_type return_all_type traverse_type : type_axioms.
 
     #[local]
     Hint Resolve scan_vertices_wf filter_vertices_by_label_wf filter_edges_by_label_wf
-                 expand_all_wf expand_into_wf return_all_wf : wf_axioms.
+                 expand_all_wf expand_into_wf return_all_wf traverse_wf : wf_axioms.
 
     Section eval.
       Variable graph : PropertyGraph.t.
@@ -266,6 +298,8 @@ Module ExecutionPlan.
         | Expand mode n_from n_edge n_to d plan => 
           eval plan >>= expand mode n_from n_edge n_to d graph
         | ReturnAll plan => eval plan >>= return_all graph
+        | Traverse slice n_from plan =>
+          eval plan >>= traverse slice n_from graph
         end.
     End eval.
 
@@ -293,463 +327,3 @@ Module ExecutionPlan.
     Qed.
   End EvalPlan.
 End ExecutionPlan.
-
-Module ExecutionPlanImpl : ExecutionPlan.Spec.
-
-  Definition scan_vertices (n : Name.t)
-                           (graph : PropertyGraph.t) :
-    option BindingTable.t :=
-    Some (map (fun v => n |-> Value.GVertex v) (vertices graph)).
-
-  Section filter_by_label.
-    Variable mode : FilterMode.t.
-    Variable n : Name.t.
-    Variable l : PropertyGraph.label.
-    Variable graph : PropertyGraph.t.
-    Variable table : BindingTable.t.
-
-    Definition vertex_has_label (r : Rcd.t) : bool :=
-      match r n with
-      | Some (Value.GVertex v) => In_decb l (vlabels graph v)
-      | _ => false
-      end.
-
-    Definition edge_has_label (r : Rcd.t) : bool :=
-      match r n with
-      | Some (Value.GEdge e) => elabel graph e ==b l
-      | _ => false
-      end.
-
-    Definition has_label : Rcd.t -> bool :=
-      match mode with
-      | Vertices => vertex_has_label
-      | Edges => edge_has_label
-      end.
-
-    Definition filter_by_label : option BindingTable.t :=
-      Some (filter has_label table).
-  End filter_by_label.
-
-  #[local]
-  Hint Unfold filter_by_label has_label vertex_has_label edge_has_label : filter_by_label_db.
-
-  Section expand.
-    Variable mode : ExpandMode.t.
-    Variable n_from n_edge n_to : Name.t.
-    Variable d : Pattern.direction.
-    Variable graph : PropertyGraph.t.
-    Variable table : BindingTable.t.
-
-    Definition expand_all_single (r : Rcd.t) : option BindingTable.t :=
-      match r n_from, r n_edge, r n_to with
-      | Some (Value.GVertex v_from), None, None =>
-        Some (map (fun '(e, v_to) => n_to   |-> Value.GVertex v_to;
-                                     n_edge |-> Value.GEdge e; r)
-          match d with
-          | Pattern.OUT  => out_edges graph v_from
-          | Pattern.IN   => in_edges  graph v_from
-          | Pattern.BOTH => out_edges graph v_from ++
-                            in_edges  graph v_from
-          end)
-      | _, _, _ => None
-      end.
-
-    Definition expand_into_single (r : Rcd.t) : option BindingTable.t :=
-      match r n_from, r n_edge, r n_to with
-      | Some (Value.GVertex v_from), None, Some (Value.GVertex v_to) =>
-          Some (map (fun e => n_to   |-> Value.GVertex v_to;
-                              n_edge |-> Value.GEdge e; r)
-          match d with
-          | Pattern.OUT  => edges_between graph v_from v_to
-          | Pattern.IN   => edges_between graph v_to   v_from
-          | Pattern.BOTH => edges_between graph v_from v_to ++
-                            edges_between graph v_to   v_from
-          end)
-      | _, _, _ => None
-      end.
-
-    Definition expand_single (r : Rcd.t) : option BindingTable.t :=
-      match mode with
-      | All => expand_all_single r
-      | Into => expand_into_single r
-      end.
-
-    Definition expand : option BindingTable.t :=
-      option_map (@List.concat Rcd.t) (fold_option (map expand_single table)).
-  End expand.
-
-  #[local]
-  Hint Unfold expand expand_single expand_all_single expand_into_single : expand_db.
-
-  Definition return_all (graph : PropertyGraph.t) (table : BindingTable.t) :=
-    Some (map Rcd.explicit_proj table).
-
-  (** If the inputs are well-formed then the operation will return the result *)
-
-  Theorem scan_vertices_wf graph n (Hwf : PropertyGraph.wf graph) :
-    exists table', scan_vertices n graph = Some table'.
-  Proof using. now eexists. Qed.
-
-  Theorem filter_by_label_wf graph table ty mode n l
-                             (Hwf : PropertyGraph.wf graph)
-                             (Htype : BindingTable.of_type table ty)
-                             (Hty : match mode with
-                                    | Vertices => ty n = Some Value.GVertexT
-                                    | Edges    => ty n = Some Value.GEdgeT
-                                    end) :
-    exists table', filter_by_label mode n l graph table = Some table'.
-  Proof using.
-    autounfold with filter_by_label_db.
-    all: induction table as [| r table IH]; ins; eauto.
-  Qed.
-
-  Theorem filter_vertices_by_label_wf graph table ty n l
-                                    (Hwf : PropertyGraph.wf graph)
-                                    (Htype : BindingTable.of_type table ty)
-                                    (Hty : ty n = Some Value.GVertexT) :
-    exists table', filter_by_label Vertices n l graph table = Some table'.
-  Proof using. eapply filter_by_label_wf with (mode := Vertices); eassumption. Qed.
-
-  Theorem filter_edges_by_label_wf graph table ty n l
-                                 (Hwf : PropertyGraph.wf graph)
-                                 (Htype : BindingTable.of_type table ty)
-                                 (Hty : ty n = Some Value.GEdgeT) :
-    exists table', filter_by_label Edges n l graph table = Some table'.
-  Proof using. eapply filter_by_label_wf with (mode := Edges); eassumption. Qed.
-
-  Theorem expand_wf graph table ty mode n_from n_edge n_to d
-                    (Hwf : PropertyGraph.wf graph)
-                    (Htype : BindingTable.of_type table ty)
-                    (Hty_from : ty n_from = Some Value.GVertexT)
-                    (Hty_edge : ty n_edge = None)
-                    (Hty_to   : match mode with
-                                | All => ty n_to = None
-                                | Into => ty n_to = Some Value.GVertexT 
-                                end) :
-    exists table', expand mode n_from n_edge n_to d graph table = Some table'.
-  Proof using.
-    all: autounfold with expand_db.
-    
-    eenough (exists t, fold_option _ = Some t) as [t Hfold].
-    { rewrite Hfold. now eexists. }
-
-    apply fold_option_some; intros a HIn; simpls.
-    apply in_map_iff in HIn as [r [? ?]]; subst.
-
-    edestruct BindingTable.type_of_GVertexT with (k := n_from) as [v_from Hv_from];
-      try eassumption.
-    rewrite Hv_from.
-
-    destruct mode.
-    2: edestruct BindingTable.type_of_GVertexT with (k := n_to) as [v_to Hv_to];
-        try eassumption.
-    2: rewrite Hv_to.
-    all: repeat erewrite BindingTable.type_of_None; try eassumption.
-    all: now eexists.
-  Qed.
-
-  Theorem expand_all_wf graph table ty n_from n_edge n_to d
-                  (Hwf : PropertyGraph.wf graph)
-                  (Htype : BindingTable.of_type table ty)
-                  (Hty_from : ty n_from = Some Value.GVertexT)
-                  (Hty_edge : ty n_edge = None)
-                  (Hty_to   : ty n_to   = None) :
-    exists table', expand All n_from n_edge n_to d graph table = Some table'.
-  Proof using. eapply expand_wf with (mode := All); eassumption. Qed.
-
-  Theorem expand_into_wf graph table ty n_from n_edge n_to d
-                  (Hwf : PropertyGraph.wf graph)
-                  (Htype : BindingTable.of_type table ty)
-                  (Hty_from : ty n_from = Some Value.GVertexT)
-                  (Hty_edge : ty n_edge = None)
-                  (Hty_to   : ty n_to   = Some Value.GVertexT) :
-    exists table', expand Into n_from n_edge n_to d graph table = Some table'.
-  Proof using. eapply expand_wf with (mode := Into); eassumption. Qed.
-
-  Theorem return_all_wf graph table :
-    exists table', return_all graph table = Some table'.
-  Proof using. now eexists. Qed.
-
-  (** If the operation returned some table then the type of the table is correct *)
-  
-  Theorem scan_vertices_type graph table' n 
-                           (Hres : scan_vertices n graph = Some table') :
-    BindingTable.of_type table' (n |-> Value.GVertexT).
-  Proof using.
-    unfold scan_vertices in Hres.
-    injection Hres as Hres. subst. intros r' HIn.
-    apply in_map_iff in HIn as [r [Heq HIn]].
-    subst.
-    solve_type_of.
-  Qed.
-  
-  Theorem filter_by_label_type graph table table' ty mode n l
-                             (Hres : filter_by_label mode n l graph table = Some table')
-                             (Htype : BindingTable.of_type table ty) :
-    BindingTable.of_type table' ty.
-  Proof using.
-    generalize dependent table'.
-    destruct mode.
-    all: autounfold with filter_by_label_db.
-    all: induction table; ins; desf; eauto with type_of_db.
-  Qed.
-
-  Theorem expand_single_type graph r table' mode n_from n_edge n_to d
-    (Hres : expand_single mode n_from n_edge n_to d graph r = Some table') :
-      BindingTable.of_type table'
-        (n_to |-> Value.GVertexT; n_edge |-> Value.GEdgeT; Rcd.type_of r).
-  Proof using.
-    autounfold with expand_db in *.
-    desf.
-    all: intros r' HIn'.
-    all: apply in_map_iff in HIn'; desf.
-    all: solve_type_of_extension r (Rcd.type_of r).
-  Qed.
-
-  Theorem expand_type graph table table' ty mode n_from n_edge n_to d
-                          (Hres : expand mode n_from n_edge n_to d graph table = Some table')
-                          (Htype : BindingTable.of_type table ty) :
-    BindingTable.of_type table'
-      (n_to |-> Value.GVertexT; n_edge |-> Value.GEdgeT; ty).
-  Proof using.
-    unfold expand in *.
-    unfold option_map in Hres; desf.
-    destruct mode.
-
-    all: apply BindingTable.of_type_concat; intros table' HIn_tables'.
-    all: eassert (Hmap : In (Some table') (map _ table))
-          by (eapply fold_option_In; eauto).
-
-    all: apply in_map_iff in Hmap as [r ?]; desf.
-    all: assert (Rcd.type_of r = ty) as Hty by auto; subst.
-    all: eauto using expand_single_type.
-  Qed.
-
-  Theorem return_all_type graph table table' ty
-                          (Hres : return_all graph table = Some table')
-                          (Htype : BindingTable.of_type table ty) :
-    BindingTable.of_type table' (Rcd.explicit_projT ty).
-  Proof using.
-    intros r' HIn.
-    unfold return_all in Hres.
-    injection Hres as ?; subst.
-    apply in_map_iff in HIn as [r [? HIn]]; subst.
-    rewrite Rcd.type_of_explicit_proj.
-    now rewrite Htype with r.
-  Qed.
-
-  (** scan_vertices specification *)
-
-  
-  Theorem scan_vertices_spec graph table' n v
-    (Hres : scan_vertices n graph = Some table')
-    (HIn : In v (vertices graph)) :
-      In (n |-> Value.GVertex v) table'.
-  Proof using.
-    unfold scan_vertices in Hres.
-    inj_subst.
-    apply in_map_iff.
-    exists v. auto.
-  Qed.
-
-  Theorem scan_vertices_spec' graph table' n r'
-    (Hres : scan_vertices n graph = Some table')
-    (HIn : In r' table') :
-      exists v, r' = (n |-> Value.GVertex v) /\ In v (vertices graph).
-  Proof using.
-    unfold scan_vertices in Hres.
-    inj_subst.
-    apply in_map_iff in HIn as [v [Heq HIn]].
-    subst. exists v. auto.
-  Qed.
-
-  (** filter_by_label specification *)
-
-  Theorem vertex_has_label_true_iff graph n l r :
-    vertex_has_label n l graph r = true <->
-      exists v, r n = Some (Value.GVertex v) /\ In l (vlabels graph v).
-  Proof using.
-    split; ins.
-    all: unfold vertex_has_label in *.
-    all: desf; normalize_bool.
-    { eexists. split; eauto. }
-    now rewrite -> In_decb_true_iff.
-  Qed.
-
-  Theorem edge_has_label_true_iff graph n l r :
-    edge_has_label n l graph r = true <->
-      exists e, r n = Some (Value.GEdge e) /\ elabel graph e = l.
-  Proof using.
-    split; ins.
-    all: unfold edge_has_label in *.
-    all: desf.
-    { eexists. split. { eauto. }
-      now rewrite <- equiv_decb_true_iff. }
-    now rewrite -> equiv_decb_true_iff.
-  Qed.
-
-  Theorem filter_by_label_spec graph table table' mode n l r 
-    (Hres : filter_by_label mode n l graph table = Some table') :
-      match mode with
-      | Vertices => In r table' <-> In r table /\
-          (exists v, r n = Some (Value.GVertex v) /\ In l (vlabels graph v))
-      | Edges    => In r table' <-> In r table /\
-          (exists e, r n = Some (Value.GEdge e) /\ elabel graph e = l)
-      end.
-  Proof using.
-    unfold filter_by_label, has_label in Hres.
-    inj_subst.
-    destruct mode; ins.
-    all: rewrite filter_In.
-    1: rewrite -> vertex_has_label_true_iff; try eassumption.
-    2: rewrite -> edge_has_label_true_iff; try eassumption.
-    all: reflexivity.
-  Qed.
-
-  Theorem filter_vertices_by_label_spec graph table table' n l v r 
-    (Hres : filter_by_label Vertices n l graph table = Some table')
-    (Hval : r n = Some (Value.GVertex v)) (Hlabel : In l (vlabels graph v))
-    (HIn : In r table) : In r table'.
-  Proof using.
-    rewrite -> filter_by_label_spec with (mode := Vertices); eauto.
-  Qed.
-  
-  Theorem filter_vertices_by_label_spec' graph table table' n l r' 
-    (Hres : filter_by_label Vertices n l graph table = Some table')
-    (HIn : In r' table') : In r' table /\
-        exists v, r' n = Some (Value.GVertex v) /\ In l (vlabels graph v).
-  Proof using.
-    rewrite <- filter_by_label_spec with (mode := Vertices); eauto.
-  Qed.
-
-  Theorem filter_edges_by_label_spec graph table table' n l e r 
-    (Hres : filter_by_label Edges n l graph table = Some table')
-    (Hval : r n = Some (Value.GEdge e)) (Hlabel : elabel graph e = l)
-    (HIn : In r table) : In r table'.
-  Proof using.
-    rewrite -> filter_by_label_spec with (mode := Edges); eauto.
-  Qed.
-  
-  Theorem filter_edges_by_label_spec' graph table table' n l r' 
-    (Hres : filter_by_label Edges n l graph table = Some table')
-    (HIn : In r' table') : In r' table /\
-        exists e, r' n = Some (Value.GEdge e) /\ elabel graph e = l.
-  Proof using.
-    rewrite <- filter_by_label_spec with (mode := Edges); eauto.
-  Qed.
-  
-  (** expand specification *)
-
-  Theorem expand_single_spec graph table' r r' mode n_from n_edge n_to d
-    (Hres : expand_single mode n_from n_edge n_to d graph r = Some table') :
-      expansion_of graph r' r mode n_from n_edge n_to d <-> In r' table'.
-  Proof using.
-    split; ins.
-    all: unfold expansion_of, expansion_of', Path.matches_direction in *.
-
-    - destruct mode; desf.
-      all: autounfold with expand_db in Hres.
-      all: rewrite Hval_from, Hval_to in Hres; desf.
-      all: apply in_map_iff.
-      all: try exists (e, v_to).
-      all: try exists e.
-      all: split; [ reflexivity | ].
-      all: try apply in_or_app.
-      all: try rewrite -> in_edges_In.
-      all: try rewrite -> out_edges_In.
-      all: repeat rewrite -> edges_between_In.
-      all: unfold e_from, e_to; destruct (ends graph e); desf.
-      all: auto.
-
-    - all: autounfold with expand_db in Hres.
-      destruct mode; desf.
-      all: match goal with
-           | [ H : In _ (map _ _) |- _ ] => apply in_map_iff in H; desf
-           end.
-      all: try match goal with
-           | [ H : In _ (_ ++ _) |- _ ] => apply in_app_or in H
-           end; desf.
-      all: match goal with
-           | [ H : In _ (out_edges       _ _) |- _ ] =>
-               apply out_edges_In in H
-           | [ H : In _ (in_edges        _ _) |- _ ] =>
-               apply in_edges_In in H
-           | [ H : In _ (edges_between _ _ _) |- _ ] =>
-               apply edges_between_In in H
-           end; desf.
-      all: do 3 eexists.
-      all: splits; eauto.
-
-      all: unfold e_from, e_to in *; edestruct (ends graph _); desf; simpls.
-      all: auto.
-  Qed.
-
-  Theorem expand_spec graph table table' r r' mode n_from n_edge n_to d
-      (Hres : expand mode n_from n_edge n_to d graph table = Some table')
-      (Hexp : expansion_of graph r' r mode n_from n_edge n_to d)
-      (HIn : In r table) : In r' table'.
-  Proof using.
-    unfold expand in *.
-
-    edestruct (fold_option _) as [tables' | ] eqn:Hfold.
-    2: now inv Hres.
-    simpls; inj_subst.
-
-    eassert (Hmap : In (_ r) (map _ table)) by (now eapply in_map).
-
-    eassert (exists table', _ r = Some table') as [table' Hres].
-    { eapply fold_option_some_inv in Hfold as [table' Heq]; eauto. }
-
-    apply in_concat. exists table'. split.
-    2: now eapply expand_single_spec; eauto.
-    eapply fold_option_In; eauto.
-    unfold BindingTable.t in *.
-    now rewrite <- Hres.
-  Qed.
-
-  Theorem expand_spec' graph table table' r' mode n_from n_edge n_to d
-    (Hres : expand mode n_from n_edge n_to d graph table = Some table')
-    (HIn : In r' table') :
-      exists r, In r table /\
-                expansion_of graph r' r mode n_from n_edge n_to d.
-  Proof using.
-    unfold expand in *.
-    edestruct (fold_option _) as [tables' | ] eqn:?.
-    2: now inv Hres.
-    simpls; inj_subst.
-
-    apply in_concat in HIn as [table' ?]; desf.
-    eassert (Hmap : In (Some table') (map _ table)).
-    { eapply fold_option_In; eassumption. }
-
-    apply in_map_iff in Hmap as [r ?]; desf.
-    exists r. split.
-    { assumption. }
-    eapply expand_single_spec; eassumption.
-  Qed.
-
-  (* return_all specification *)
-
-  Theorem return_all_spec graph table table' r
-    (Hres : return_all graph table = Some table')
-    (HIn : In r table) :
-      In (Rcd.explicit_proj r) table'.
-  Proof using.
-    unfold return_all in *.
-    injection Hres as ?; subst.
-    eapply in_map in HIn.
-    eassumption.
-  Qed.
-
-  Theorem return_all_spec' graph table table' r'
-    (Hres : return_all graph table = Some table')
-    (HIn : In r' table') :
-      exists r, In r table /\ r' = Rcd.explicit_proj r.
-  Proof using.
-    unfold return_all in *.
-    injection Hres as ?; subst.
-    apply in_map_iff in HIn as [r ?]; desf.
-    eauto.
-  Qed.
-End ExecutionPlanImpl.
-
