src/TraverseOp.v
@@ -1,0 +1,53 @@
+Require Import String.
+Require Import List.
+Require Import Bool.
+Require Import BinNums.
+From Coq Require Import Logic.FunctionalExtensionality.
+Import ListNotations.
+
+Require Import Maps.
+Require Import Utils.
+Require Import PropertyGraph.
+Require Import Cypher.
+Require Import BindingTable.
+Require Import Semantics.
+Require Import PatternE.
+Require Import ExecutionPlan.
+
+Import PartialMap.Notations.
+Import TotalMap.Notations.
+Import PropertyGraph.
+Import ExecutionPlan.
+Import FilterMode.
+Import ExpandMode.
+Import MatchMode.
+Import UpdateNotations.
+
+Module TraverseOpImpl.
+  Definition traverse : PatternSlice.t -> Name.t -> step1.
+  Admitted.
+
+  Theorem traverse_wf : forall graph table ty slice n_from,
+    PropertyGraph.wf graph -> BindingTable.of_type table ty ->
+      PatternSlice.wf ty slice -> ty n_from = Some Value.GVertexT ->
+        exists table', traverse slice n_from graph table = Some table'.
+  Admitted.
+
+  Theorem traverse_type : forall graph table table' ty slice n_from,
+    traverse slice n_from graph table = Some table' ->
+      BindingTable.of_type table ty ->
+        BindingTable.of_type table' (PatternSlice.type_of ty slice).
+  Admitted.
+
+  Theorem traverse_spec : forall graph table table' path r r' slice n_from,
+    traverse slice n_from graph table = Some table' ->
+      PathSlice.matches graph r n_from r' path slice ->
+        In r table -> In r' table'.
+  Admitted.
+
+  Theorem traverse_spec' : forall graph table table' r' slice n_from,
+    traverse slice n_from graph table = Some table' ->
+      In r' table' -> exists r path, In r table /\
+        PathSlice.matches graph r n_from r' path slice.
+  Admitted.
+End TraverseOpImpl.
